Work in ffi/ByteStringFFI.v

ffi/ByteStringFFI.v
@@ -1,3 +1,167 @@
+Require Import
+  ByteString.Lib.Tactics
+  ByteString.Lib.Nomega
+  ByteString.Lib.Fiat
+  ByteString.Lib.TupleEnsembles
+  ByteString.Lib.FunMaps
+  ByteString.Memory
+  ByteString.Heap
+  ByteString.FFI.HeapFFI
+  ByteString.ByteString
+  ByteString.ByteStringHeap
+  Coq.FSets.FMapFacts
+  Coq.Structures.DecidableTypeEx
+  Hask.Data.Functor
+  Hask.Control.Monad
+  Hask.Control.Monad.Free.
+
+Module ByteStringFFI (M : WSfun N_as_DT).
+
+Module Import ByteStringHeap := ByteStringHeap M.
+Module Import HeapFFI := HeapFFI M.
+
+Import HeapCanonical.
+Import FunMaps.
+Import Heap.
+Import HeapState.
+Import FMapExt.
+
+Section Refined.
+
+Inductive HeapF (r : Type) : Type :=
+  | Empty   : HeapF r
+  | Alloc   : forall (len : Size | 0 < len) (k : N -> r), HeapF r
+  | Free_   : forall (addr : Ptr), r -> HeapF r
+  | Realloc : forall (addr : Ptr) (len : Size | 0 < len) (k : N -> r), HeapF r
+  | Peek    : forall (addr : Ptr) (k : Word -> r), HeapF r
+  | Poke    : forall (addr : Ptr) (w : Word), r -> HeapF r
+  | Memcpy  : forall (addr : Ptr) (addr2 : Ptr) (len : Size), r -> HeapF r
+  | Memset  : forall (addr : Ptr) (len : Ptr) (w : Word), r -> HeapF r.
+
+Program Instance HeapF_Functor : Functor HeapF := {
+  fmap := fun _ _ f x =>
+    match x with
+    | Empty                   => Empty _
+    | Alloc len k             => Alloc len (compose f k)
+    | Free_ addr x            => Free_ addr (f x)
+    | Realloc addr len k      => Realloc addr len (compose f k)
+    | Peek addr k             => Peek addr (compose f k)
+    | Poke addr w x           => Poke addr w (f x)
+    | Memcpy addr addr2 len x => Memcpy addr addr2 len (f x)
+    | Memset addr len w x     => Memset addr len w (f x)
+    end
+}.
+
+Definition HeapDSL := Free HeapF.
+
+Inductive MonadRefinement `{Monad m} : forall (A B : Type) (AbsR : A -> B -> Prop),
+  Comp A -> m B -> Prop :=
+  | MBind A B (AbsR : A -> B -> Prop) :
+      forall c c', MonadRefinement AbsR c c'
+        -> forall k k',
+             (forall v v', AbsR v v' -> MonadRefinement AbsR (k v) (k' v'))
+        -> MonadRefinement AbsR (c >>= k)%comp (c' >>= k')%monad
+  | MReturn A B (AbsR : A -> B -> Prop) x x' :
+      AbsR x x'
+        -> MonadRefinement AbsR (ret x)%comp (pure x')
+  | MRefine A B (AbsR : A -> B -> Prop) c c' d :
+      refine c' c
+        -> MonadRefinement AbsR c d
+        -> MonadRefinement AbsR c' d
+  | MIf A B (AbsR : A -> B -> Prop) b t t' e e' :
+      (b = true -> MonadRefinement AbsR t t')
+        -> (b = false -> MonadRefinement AbsR e e')
+        -> MonadRefinement AbsR (If b Then t Else e)%comp (if b then t' else e').
+
+Definition matchPS {A B : Type} (r : PS A) (r' : PS B) : Prop :=
+  psBuffer r = psBuffer r' /\
+  psBufLen r = psBufLen r' /\
+  psOffset r = psOffset r' /\
+  psLength r = psLength r'.
+
+Definition ByteString (r : Rep HeapSpec) := Rep (projT1 (ByteStringHeap r)).
+
+Definition cons (r : Rep HeapSpec) (w : Word) (bs : ByteString r) :
+  Comp (ByteString r) :=
+  Eval simpl in
+    (p <- callMeth (projT1 (ByteStringHeap r)) consS bs w; ret (fst p)).
+
+Lemma consDSL :
+  { f : Word -> PS unit -> HeapDSL (PS unit)
+  & forall r w bs bs',
+      matchPS bs bs' ->
+      MonadRefinement matchPS (cons (r:=r) w bs) (f w bs') }.
+Proof.
+  eexists.
+  intros.
+  destruct H.
+  repeat breakdown.
+  unfold cons; simpl.
+  eapply MRefine; eauto.
+    simplify with monad laws; simpl.
+    rewrite refine_If_Then_Else_Bind.
+    setoid_rewrite H1.
+    reflexivity.
+  apply MIf; intros.
+    eapply MRefine; eauto.
+      simplify with monad laws; simpl.
+      reflexivity.
+    remember (makePS _ _ _ _ _) as P.
+    apply MReturn with (x:=P)
+      (x':={| psHeap   := tt
+            ; psBuffer := psBuffer bs'
+            ; psBufLen := psBufLen bs'
+            ; psOffset := psOffset bs' - 1
+            ; psLength := psLength bs' + 1 |}); subst.
+    repeat constructor;
+    simpl in *; auto.
+      rewrite H1; reflexivity.
+    rewrite H2; reflexivity.
+  eapply MRefine; eauto.
+    rewrite refine_If_Then_Else_Bind.
+    setoid_rewrite H2.
+    setoid_rewrite H0.
+    reflexivity.
+  apply MIf; intros.
+    unfold make_room_by_shifting_up.
+    eapply MRefine; eauto.
+      rewrite refine_bind_bind.
+      setoid_rewrite refine_bind_unit at 2.
+      simpl.
+      reflexivity.
+    instantiate (1 := liftF (Memcpy (psBuffer bs') (psBuffer bs' + 1)
+                                    (psLength bs') bs')).
+    admit.
+  eapply MRefine; eauto.
+    rewrite refine_If_Then_Else_Bind.
+    reflexivity.
+  apply MIf; intros.
+    unfold make_room_by_growing_buffer, Bind2; simpl.
+    eapply MRefine; eauto.
+      rewrite refine_bind_bind.
+      setoid_rewrite refine_bind_bind at 2.
+      setoid_rewrite refine_bind_bind at 2.
+      setoid_rewrite refine_bind_unit at 3; simpl.
+      unfold ByteStringHeap.buffer_cons_obligation_2.
+      reflexivity.
+    admit.
+  unfold allocate_buffer, Bind2; simpl.
+  eapply MRefine; eauto.
+    rewrite refine_bind_bind.
+    setoid_rewrite refine_bind_unit at 1.
+    unfold ByteStringHeap.buffer_cons_obligation_3.
+    simpl.
+    reflexivity.
+  admit.
+Admitted.
+
+Definition consDSL' := Eval simpl in projT1 consDSL.
+Print consDSL'.
+
+End Refined.
+
+End ByteStringFFI.
+
 (** This is the code we intend to approximate with the FFI refined version of
     ByteString:
 
